theories/case_studies/multiuser_kvs/kvs_spec_read.v
@@ -9,7 +9,7 @@ Section KVS_spec_read.
     {Σ:gFunctors}
     {ceriseg:ceriseG Σ} {sealsg: sealStoreG Σ}
     {Cname : CmptNameG}
-    {stsg : STSG Addr region_type Σ} {heapg : heapGS Σ}
+    {stsg : STSG Addr region_type OType Word Σ} {heapg : heapGS Σ}
     {kvsg:kvsG Σ}
     {nainv: logrel_na_invs Σ}
     {cstackg : CSTACKG Σ}
